Some library code for attribute accesses (not yet working)
RegExp Expression Inner Syntax defined

RexExp Parsing activated.

RegExp.thy
@@ -1,25 +1,23 @@
 theory RegExp
 imports Main 
 begin
-
+value "insert"
+  
 datatype 'a rexp = Empty                         ("<>")
                  | Atom 'a                       ("\<lfloor>_\<rfloor>" 65)
-                 | Alt  "('a rexp)" "('a rexp)"  (infix "|" 55)
-                 | Conc "('a rexp)" "('a rexp)"  (infix ":" 60)
-                 | Star "('a rexp)"              
+                 | Alt  "('a rexp)" "('a rexp)"  (infixr "||" 55)
+                 | Conc "('a rexp)" "('a rexp)"  (infixr "~~" 60)
+                 | Star "('a rexp)"              ("\<lbrace>(_)\<rbrace>\<^sup>*" [0]100)          
 
-
+definition rep1 :: "'a rexp \<Rightarrow> 'a rexp" ("\<lbrace>(_)\<rbrace>\<^sup>+")
+  where "\<lbrace>A\<rbrace>\<^sup>+ \<equiv>  A ~~ \<lbrace>A\<rbrace>\<^sup>*"
+    
+definition opt :: "'a rexp \<Rightarrow> 'a rexp" ("\<lbrakk>(_)\<rbrakk>")
+   where "\<lbrakk>A\<rbrakk> \<equiv>  A || <>"
+                   
 value "Star (Conc(Alt (Atom(CHR ''a'')) (Atom(CHR ''b''))) (Atom(CHR ''c'')))"
 text{* or better equivalently: *}
-value "Star ((\<lfloor>CHR ''a''\<rfloor> | \<lfloor>CHR ''b''\<rfloor>) : \<lfloor>CHR ''c''\<rfloor>)"
-
-text{* Let's try to prove something obvious : *}
-lemma alt_commute : " ((A::'a rexp) | B) = (B | A)"   (* use the type annotation to disambiguate *)
-apply(case_tac A, simp_all)
-apply(case_tac B, simp_all)
-oops
-
-text{* This is simply FALSE. Why ??? *}
+value "\<lbrace>(\<lfloor>CHR ''a''\<rfloor> || \<lfloor>CHR ''b''\<rfloor>) ~~ \<lfloor>CHR ''c''\<rfloor>\<rbrace>\<^sup>*"
 
 
 section{* Definition of a semantic function: the ``language'' of the regular expression *}
@@ -34,11 +32,11 @@ type_synonym 'a lang = "'a list set"
 
 inductive_set star :: "'a lang \<Rightarrow> 'a lang"
               for A:: "'a lang"
-where   NilI  : "[] : star A"
-     |  ConsI : "[| a:A; as : star A |] ==> a@as : star A"
+where   NilI  : "[] \<in> star A"
+     |  ConsI : "[| a\<in>A; as \<in> star A |] ==> a@as \<in> star A"
 
 
-lemma NilI : "[] : star A"
+lemma NilI : "[] \<in> star A"
 by(rule NilI)
 
 
@@ -47,27 +45,12 @@ apply(rule ConsI)
 apply(assumption)
 by(assumption)
 
-
-find_theorems (80) name:"Set." name:"eq"
-
 lemma epsilonExists: "star {[]} = {[]}"
-apply(subst set_eq_iff)
-apply(rule allI)
-apply(rule iffI)
-apply(rule_tac A="{[]}" in  star.induct)back
-apply(assumption)
-apply simp
-apply simp
-by (simp add: star.NilI)
-
-
-lemma epsilonExists': "star {[]} = {[]}"
 apply(rule Set.set_eqI)
 apply(rule iffI)
 apply(erule star.induct)
 apply(auto intro: NilI )
 done
-
 
 lemma epsilonAlt: "star {} = {[]}"
 apply(rule Set.set_eqI)
@@ -94,12 +77,12 @@ text{* Now the denotational semantics for regular expression can be defined on a
 fun              L :: "'a rexp => 'a lang"
 where L_Emp :   "L Empty      = {}"
      |L_Atom:   "L (\<lfloor>a\<rfloor>)      = {[a]}"
-     |L_Un:     "L (el | er)  = (L el) \<union> (L er)"
-     |L_Conc:   "L (el : er)  = {xs@ys | xs ys. xs:L el \<and> ys:L er}"
+     |L_Un:     "L (el || er)  = (L el) \<union> (L er)"
+     |L_Conc:   "L (el ~~ er)  = {xs@ys | xs ys. xs:L el \<and> ys:L er}"
      |L_Star:   "L (Star e)   = star(L e)"
 
 
-schematic_goal WeCompute: "L(Star ((\<lfloor>CHR ''a''\<rfloor> | \<lfloor>CHR ''b''\<rfloor>) : \<lfloor>CHR ''c''\<rfloor>)) = ?X"
+schematic_goal WeCompute: "L(Star ((\<lfloor>CHR ''a''\<rfloor> || \<lfloor>CHR ''b''\<rfloor>) ~~ \<lfloor>CHR ''c''\<rfloor>)) = ?X"
 by simp
 
 thm WeCompute
@@ -111,45 +94,19 @@ text{* Well, an attempt to evaluate this turns out not to work too well ... *}
 text{* Now let's reconsider our `obvious lemma' from above, this time by stating that
        the alternative-operator produces \emph{semantically} equivalent ewpressions. *}  
 
-lemma alt_commute : "L((A::'a rexp) | B) = L(B | A)"
-apply(subst L_Un)
-apply(subst L_Un)
-apply(rule inf_sup_aci)
-done
 
 
-lemma alt_commute' : "L((A::'a rexp) | B) = L(B | A)"  
+lemma alt_commute' : "L((A::'a rexp) || B) = L(B || A)"  
 by auto
 
 
-lemma alt_commute'' : "L((A::'a rexp) | B) = L(B | A)"  
-using alt_commute' by blast
-
-lemma mt_seq : "L(Empty : Empty) = {}"
-apply(subst L_Conc)
-apply(subst L_Emp)
-apply(subst L_Emp)
-apply(subst Set.empty_iff)
-apply(subst  HOL.simp_thms(24))
-apply(subst Set.Collect_empty_eq)
-apply(subst HOL.simp_thms(23))
-apply(rule allI)
-apply(subst HOL.not_ex)
-apply(subst HOL.not_ex)
-apply(rule allI)
-apply(rule allI)
-apply(subst HOL.not_False_eq_True)
-apply(rule TrueI)
-done
-
-lemma mt_seq' : "L(Empty : Empty) = {}"
+lemma mt_seq' : "L(Empty ~~ Empty) = {}"
 by simp
 
 
 lemma eps : "L (Star Empty) = {[]}"
 by (simp add: epsilonAlt)
 
-  term "\<lfloor>X\<rfloor>"
   
 no_notation Atom ("\<lfloor>_\<rfloor>")  
 
